theory/Game/Strategy.v
@@ -75,3 +75,103 @@ CoInductive drawing_strategy {G : Game} (p : Player) : forall {s : GameState G},
       (strs : forall m, strategy p (exec_move s m)),
       (forall m, no_worse_strategy p (strs m)) ->
       drawing_strategy p (abelard_strategy res_pf play_pf strs).
+
+CoInductive outcome : Type :=
+  | W : Player -> outcome
+  | step : outcome -> outcome.
+
+CoFixpoint D : outcome := step D.
+
+Definition outcome_id (o : outcome) : outcome :=
+  match o with
+  | W p => W p
+  | step o => step o
+  end.
+
+Lemma outcome_id_eq (o : outcome) :
+  o = outcome_id o.
+Proof.
+  destruct o; reflexivity.
+Qed.
+
+CoFixpoint play_game {G} {p} (s : GameState G) (str_pl : strategy p s) (str_opp : strategy (opp p) s) : outcome.
+Proof.
+  destruct str_pl.
+  - destruct res.
+    + exact (W p0).
+    + exact D.
+  - destruct str_opp.
+    + congruence.
+    + elim (opp_no_fp p); congruence.
+    + apply step.
+      exact (play_game G p _ str_pl (s m)).
+  - destruct str_opp.
+    + congruence.
+    + apply step.
+      exact (play_game G p _ (s m) str_opp).
+    + elim (opp_no_fp (opp p)); congruence.
+Defined.
+
+CoInductive outcome_le : Player -> outcome -> outcome -> Prop :=
+  | W_best : forall p o, outcome_le p o (W p)
+  | W_worst : forall p o, outcome_le p (W (opp p)) o
+  | step_mon : forall p o1 o2, outcome_le p o1 o2 -> outcome_le p (step o1) (step o2).
+
+CoFixpoint outcome_le_refl : forall p o, outcome_le p o o.
+Proof.
+  intro p.
+  destruct o.
+  - destruct (player_id_or_opp_r_t p0 p); subst.
+    + apply W_best.
+    + apply W_worst.
+  - apply step_mon.
+    apply outcome_le_refl.
+Qed.
+
+Require Import Coq.Program.Equality.
+
+CoFixpoint no_worse_strategy_correct {G} (p : Player) (b : GameState G)
+  (s : strategy p b) (s' : strategy (opp p) b) : no_worse_strategy p s ->
+  outcome_le p D (play_game b s s').
+Proof.
+  intro pf.
+  rewrite outcome_id_eq.
+  unfold outcome_id.
+  unfold play_game.
+  destruct s.
+  - destruct res.
+    + inversion pf; subst.
+      apply W_best.
+    + rewrite (outcome_id_eq D) at 1.
+      unfold outcome_id.
+      unfold D.
+      apply step_mon.
+      fold D.
+      apply outcome_le_refl.
+  - destruct s'.
+    + congruence.
+    + elim (opp_no_fp p).
+      congruence.
+    + fold @play_game.
+      rewrite (outcome_id_eq D).
+      unfold outcome_id.
+      unfold D.
+      apply step_mon.
+      fold D.
+      apply no_worse_strategy_correct.
+      dependent destruction pf.
+      auto.
+  - destruct s'.
+    + congruence.
+    + fold @play_game.
+      rewrite (outcome_id_eq D).
+      unfold outcome_id.
+      unfold D.
+      apply step_mon.
+      fold D.
+      apply no_worse_strategy_correct.
+      dependent destruction pf.
+      apply H.
+    + elim (opp_no_fp (opp p)); congruence.
+Defined.
+
